SrcTranslated/FunsExternal.lean
@@ -1518,9 +1518,7 @@ axiom libcrux_hmac.hmac_sha256_tag32_spec
     (hkey : key.length ≤ U32.max)
     (hdata : data.length ≤ U32.max) :
     libcrux_hmac.hmac .Sha256 key data (some 32#usize)
-      ⦃ (r : alloc.vec.Vec U8) =>
-        libcrux_hmac.hmac .Sha256 key data (some 32#usize) = ok r ∧
-        r.length = 32 ⦄
+      ⦃ (r : alloc.vec.Vec U8) => r.length = 32 ⦄
 
 /-- [libcrux_ml_kem::constants::SHARED_SECRET_SIZE]
     Source: '/cargo/registry/src/index.crates.io-1949cf8c6b5b557f/libcrux-ml-kem-0.0.7/src/constants.rs', lines 14:0-14:35
